src/checker/Pulse.Elaborate.Core.fst
@@ -255,7 +255,7 @@ let rec elab_st_typing (#g:env)
       let body = elab_st_typing body_typing in
       mk_while (mk_abs bool_tm R.Q_Explicit inv) cond body
 
-    | T_NuWhile _ inv _ _ _ cond_typing body_typing ->
+    | T_NuWhile {} ->
       (`())
 
     | T_Par _ eL cL eR cR _ _ _ eL_typing eR_typing ->
